% !TEX root = ../main.tex
\section{The Chain Rule}


\begin{myframe}[arc=10pt,auto outer arc]
	\centering Chain Rule: $\displaystyle (f\circ g)'(x) = f'(g(x)) \times g'(x)$
\end{myframe}

\pairofprobsans%
{$\displaystyle f\left(x\right) = (x^3 + 2x - 3)^4$}{$\displaystyle 4(x^3 + 2x - 3)^{3}(3x^2 + 2)$}%
{$\displaystyle f\left(x\right) = 4{\sin{(x^3)}}$}{$\displaystyle 12x^2 \cos{(x^3)}$}

\problemans%
{$\displaystyle f\left(x\right) = \frac{1}{x^3 + 2x - 3}$}{$\displaystyle -\frac{3x^2 + 2}{(x^3 + 2x - 3)^2}$}%

%%%% GUIDES
\qrfigure{chapter2/qr/Chain-Rule}{Scan for guides}